# Rewriting functions using folds

- [Rewriting functions using folds](#rewriting-functions-using-folds)
  - [and](#and)
    - [Direct recursion, not point-free](#direct-recursion-not-point-free)
    - [Folding and point-free](#folding-and-point-free)
  - [or](#or)
    - [Direct recursion, not point free](#direct-recursion-not-point-free-1)
    - [Direct recursion, point-free](#direct-recursion-point-free)
  - [any](#any)
    - [Direct recursion, not point-free](#direct-recursion-not-point-free-2)
    - [Type checking problem](#type-checking-problem)
    - [Composing with f and map](#composing-with-f-and-map)
    - [Composing (||) and f](#composing-and-f)
  - [elem](#elem)
    - [Using fold and a lambda](#using-fold-and-a-lambda)
    - [Using any](#using-any)
  - [reverse](#reverse)
    - [foldr and lambda](#foldr-and-lambda)
    - [foldl and flip (:)](#foldl-and-flip-)
  - [map](#map)
    - [using foldr and lambda](#using-foldr-and-lambda)
  - [filter](#filter)
    - [using foldr and guards](#using-foldr-and-guards)
    - [using foldr and case of](#using-foldr-and-case-of)
    - [using foldr with if else](#using-foldr-with-if-else)
  - [squish (flatten)](#squish-flatten)
    - [using foldr](#using-foldr)

## and

### Direct recursion, not point-free

```hs
myAnd :: [Bool] -> Bool
myAnd [] = True
myAnd (x:xs) = x && myAnd_r xs
```

Using `foldr`, not point free.
```hs
myAnd :: [Bool] -> Bool
myAnd = foldr (\e acc -> e && acc) True
```

### Folding and point-free

`(&&)` is the folding function and `True` is the *zero* (initial value for the accumulator). We partially apply `foldr` with the first two params. The remaining one, the list to be operated on is still missing, and it is not defined as a parameter to `myAnd`. There is no `myAnd xs = ...`. That is what makes it *point free*. The type signature denounces that wee need a list of bool, though, and return a bool.

```hs
myAnd :: [Bool] -> Bool
myAnd = foldr (&&) True
```

## or

### Direct recursion, not point free

```hs
myOr :: [Bool] -> Bool
myOr [] = False
myOr (x:xs) = x || myOr xs
```

@TODO: Why does the author say it is **not** point free? We are not declaring that `myOr` explicitly takes a list, like `myOr xs = ...`.

To me, this is point-free.

```hs
myOr :: [Bool] -> Bool
myOr = foldr (\e acc -> e || acc) False
```

Or, the folding function is not point-free, because it takes explicit params `e` and `acc`.

This is not point free because we are explicitly declaring the param `xs`.

```hs
myOr :: [Bool] -> Bool
myOr xs = foldr (\e acc -> e || acc) False xs
```

### Direct recursion, point-free

And the fully point-free version using folds.

```hs
myOr :: [Bool] -> Bool
myOr = foldr (||) False
```

“Point” in *point-free* refers to variables. Variables are the *points*. If a function mentions variables, it is not point-free.

## any

### Direct recursion, not point-free

```hs
myAny :: (a -> Bool) -> [a] -> Bool
myAny _ [] = False
myAny f (x:xs) = f x || myAny f xs
```

### Type checking problem

This version works if we comment the type signature for the inner function `g`. That type definition seems totally OK but it doesn't type check.

```hs
myAny :: (a -> Bool) -> [a] -> Bool
myAny f = foldr g False
  where
    -- g :: a -> Bool -> Bool
    g = \ x acc -> f x || acc
```

In the  definition of `g` we reference a variable that appears in the signature of `myAny`. But those `a`s are different. We could enable `ScopedTypeVariables` extension, though, which makes those `a`'s be the same.

Also, we see a compiler error mentioning `a1`, which is the name to compiler gives to the `a` polymorphic type variable in `g` to differentiate it from the `a` polymorphic type variable in `myAny`. This works:

```hs
{-# LANGUAGE ScopedTypeVariables #-}
{-# LANGUAGE ExplicitForAll #-}

myAny :: forall a. (a -> Bool) -> [a] -> Bool
myAny f = foldr g False
  where
    g :: a -> Bool -> Bool
    g = \ e acc -> f e || acc
```

Thanks @infixl-1 (Izuzu#5593) for the [help on Discord](https://discord.com/channels/280033776820813825/796099254937845790/871017722761322516). He mentioned that “I usually reserve type signatures for top-level declarations because of shenanigans like this (which honestly aren't really shenanigans).”

### Composing with f and map

```hs
myAny :: (a -> Bool) -> [] a -> Bool
myAny f = foldr (||) False . map f
```

We can think of it like this:

We first `map f` over the list of values. Ex:

```hs
λ> map even [0, 2, 3]
[True,True,False]
```

Then, we `(||)` each on the results of the previous operation:

```GHCi
λ> foldr (||) False [True, True, False]
True
```

**EXCEPT THAT BECAUSE OF LAZY EVALUATION, `map f` will only produce values as as needed by `foldr`**. It WILL NOT actually map over the entire input unless `foldr` folding function keeps asking for more values and ends up reaching the base case. As soon as `f` produces `True` for an element, `myAny` returns `True` and no more of the list is processed.

Thanks @konsumlamm for [this answer on Discord](https://discord.com/channels/280033776820813825/796099254937845790/871041627060334632).

### Composing (||) and f

This is a suggestions from the linter. Easier to understand!

```hs
myAny :: (a -> Bool) -> [] a -> Bool
myAny f = foldr ((||) . f) False
```

## elem

### Using fold and a lambda

```hs
myElem :: Eq a => a -> [a] -> Bool
myElem e = foldr (\x acc -> x == e || acc) False
```

### Using any

Partially applying `any`. Also partially applying `==`.

```hs
myElem :: Eq a => a -> [a] -> Bool
myElem e = any (e ==)
```

## reverse

### foldr and lambda

Inside the lambda, we keep concatenating the element to the end of the list. That is what reverses it.

```hs
myRev :: [a] -> [a]
myRev = foldr (\e acc -> acc ++ [e]) []
```

### foldl and flip (:)

```hs
myRev :: [a] -> [a]
myRev = foldl (flip (:)) []
```

Let's try to understand what is going on here.

```GHCi
λ> f = flip (:)

λ> :t f
f :: [a] -> a -> [a]

λ> :t (:)
(:) :: a -> [a] -> [a]

λ> [] `f` 1
[1]

λ> 1 : []
[1]
```

Both `:` and `f` add an element to the beginning of the list. But whereas `:` takes an element and a list, `f` takes a list and an element.

Not here that the list comes first, then the infix `f`, then the element:

```GHCi
λ> [1, 2] `f` 3
[3,1,2]
```

A simple implementation of `foldl` to help visualize:

```hs
foldl :: (b -> a -> b) -> b -> [] a -> b
foldl _ z [] = z
foldl f z (x:xs) = foldl f (f z x) xs
```

And a definition of `myRev` using `foldl` and `f` (which is `flip (:)`):

Here's how evaluation goes:

```GHCi
myRev = foldl f []

myRev [1, 2, 3]
foldl f ([] `f` 1) [2, 3]
→ Add 1 to the front of the acc []
→ acc now is [1]

foldl f ([1] `f` 2) [3]
→ Add 2 to the front of the acc [1]
→ acc now is [2, 1]

foldl f ([2, 1] `f` 3) []
→ Add 3 to the front of the acc [2, 1]
→ acc now is [3, 2, 1]
```

## map

### using foldr and lambda

```hs
myMap :: (a -> b) -> [a] -> [b]
myMap f = foldr (\e acc -> f e : acc) []
```

In `f e : acc`, we apply `f` to `e` producing the new value, which is then consed into `acc`.

## filter

### using foldr and guards

```hs
myFilter :: (a -> Bool) -> [a] -> [a]
myFilter f = foldr go []
  where
    go e acc
      | f e = e : acc
      | otherwise = acc
```

We could replace this line:

```
myFilter f elems = foldr go [] elems
```

```
myFilter f = foldr go []
```

That is, we partially apply `foldr` to the folding function and the accumulator, but omit the list of elements to be processed. This way, we can also omit the list of elements from `myFilter f xs`, making it just `myFilter f`.

### using foldr and case of

This indentation looks ugly.

```hs
myFilter :: (a -> Bool) -> [a] -> [a]
myFilter f =
  foldr (\e acc
    -> case f e of
        True -> e : acc
        _    -> acc) []
```

Perhaps, instead of a lambda using a run function looks better?

```hs
myFilter :: (a -> Bool) -> [a] -> [a]
myFilter f = foldr run []
  where
    run e acc =
      case f e of
        True -> e : acc
        _    -> acc
```

### using foldr with if else

This is a suggestion from the linter:

```hs
myFilter :: (a -> Bool) -> [a] -> [a]
myFilter f = foldr run []
  where
    run e acc = if f e then e : acc else acc
```

I still use the run function pattern above. We can also follow the linter suggestion but use a lambda and not the run function.

```hs
myFilter :: (a -> Bool) -> [a] -> [a]
myFilter f =
  foldr(\e acc -> if f e then e : acc else acc) []
```

## squish (flatten)

`squish` is a function that flattens a list:

```GHCi
λ> squish [[1], [2], [3]]
[1,2,3]

λ> concat [[1], [2], [3]]
[1,2,3]

λ> squish ["Tomb", "Raider", "1996"]
"TombRaider1996"
```

The built-in `concat` does the same thing.

### using foldr

```hs
squish :: [[a]] -> [a]
squish = foldr (\xs acc -> xs ++ acc) []
```

Can be simplified and shortened to:

```hs
squish :: [[a]] -> [a]
squish = foldr (++) []
```
